proof/garble/clonesMean.ec
@@ -4,26 +4,45 @@ require import Bool.
 require import Distr.
 require import Real.
 
-require import Hypothesis.
-require import Garble.
 require import Mean. export MReal.SumSet.
+
+require import PreProof.
+
 require import ReductionAda.
+
+lemma DkcExp : forall (M<:DKCS.Exp),
+  equiv[M.work~M.work:(glob M){1}=(glob M){2}==>res{1}=res{2}]
+by (intros _;fun true;progress assumption).
 
 clone Mean as MeanBool with
   type base = bool,
   op d = Dbool.dbool,
   op support = add false (add true empty)
-  proof in_support by smt.
+  proof in_support
+  by (intros=> x;delta support d;rewrite ! mem_add;case x=> ? /=;apply Dbool.supp_def).
 
 clone Mean as MeanInt with
   type base = int,
-  op d = Dinter.dinter 0 (bound-1),
-  op support = interval 0 (bound-1)
-  proof in_support by smt.
+  op d = Dinter.dinter 0 (Cst.bound-1),
+  op support = interval 0 (Cst.bound-1)
+  proof in_support
+  by (intros=> x;delta support d;rewrite mem_interval Dinter.supp_def //).
 
-module DkcWorkAdv(Adv:DKC.AdvAda_t) = {
-  module Game = DKC.GameAda(DKC.Dkc, Adv)
-  module ADV = Adv(DKC.Dkc)
+module DkcWork(Adv:DKCS.AdvAda_t) : MeanBool.Worker = {
+  module Game = DKCS.GameAda(DKCS.Dkc, Adv)
+  module ADV = Adv(DKCS.Dkc)
+  fun work(x:bool) : bool = {
+    var r : bool;
+    DKCS.Dkc.b = x;
+    ADV.preInit();
+    r = Game.work();
+    return r;
+  }
+}.
+
+module DkcWorkAdv(Adv:DKCS.AdvAda_t) = {
+  module Game = DKCS.GameAda(DKCS.Dkc, Adv)
+  module ADV = Adv(DKCS.Dkc)
   fun work() : bool = {
     var r : bool;
     ADV.preInit();
@@ -32,40 +51,21 @@ module DkcWorkAdv(Adv:DKC.AdvAda_t) = {
   }
 }.
 
-module DkcWork(Adv:DKC.AdvAda_t) : MeanBool.Worker = {
-  module Game = DKC.GameAda(DKC.Dkc, Adv)
-  module ADV = Adv(DKC.Dkc)
-  fun work(x:bool) : bool = {
-    var r : bool;
-    DKC.Dkc.b = x;
-    ADV.preInit();
-    r = Game.work();
-    return r;
-  }
-}.
-
-lemma DkcExp : forall (M<:DKC.Exp),
-  equiv[M.work~M.work:(glob M){1}=(glob M){2}==>res{1}=res{2}].
-proof.
-intros _;fun true;progress assumption.
-save.
-
-
 lemma DkcWork :
   forall b,
   forall &m,
-    forall (Adv<:DKC.AdvAda_t {DKC.Dkc, DKC.Game}),
-      DKC.Dkc.b{m} = b =>
+    forall (Adv<:DKCS.AdvAda_t {DKCS.Dkc, DKCS.Game}),
+      DKCS.Dkc.b{m} = b =>
   Pr[DkcWorkAdv(Adv).work()@ &m:res] = 
     Pr[DkcWork(Adv).work(b)@ &m:res].
 proof.
   intros b &m Adv h.
   cut eq : equiv[DkcWorkAdv(Adv).work ~ DkcWork(Adv).work
-: DKC.Dkc.b{1} = x{2} /\ (glob Adv){1} = (glob Adv){2} /\ (glob DKC.GameAda(DKC.Dkc,Adv)){1} = (glob DKC.GameAda(DKC.Dkc,Adv)){2}
+: DKCS.Dkc.b{1} = x{2} /\ (glob Adv){1} = (glob Adv){2} /\ (glob DKCS.GameAda(DKCS.Dkc,Adv)){1} = (glob DKCS.GameAda(DKCS.Dkc,Adv)){2}
       ==>res{1}=res{2}];
   last equiv_deno eq;progress assumption.
   fun.
-  call (DkcExp (DKC.GameAda(DKC.Dkc, Adv))).
+  call (DkcExp (DKCS.GameAda(DKCS.Dkc, Adv))).
   call (_:
     (glob Adv){1} = (glob Adv){2} ==>
     (res{1}=res{2}/\(glob Adv){1} = (glob Adv){2})).
@@ -76,25 +76,25 @@ save.
 
 lemma DkcEsp :
   forall &m,
-    forall (Adv<:DKC.AdvAda_t {DKC.Dkc, DKC.Game}),
-      Pr[DKC.GameAda(DKC.Dkc, Adv).main()@ &m:res] = 
+    forall (Adv<:DKCS.AdvAda_t {DKCS.Dkc, DKCS.Game}),
+      Pr[DKCS.GameAda(DKCS.Dkc, Adv).main()@ &m:res] = 
         (Pr[DkcWork(Adv).work(true)@ &m:res] +
            Pr[DkcWork(Adv).work(false)@ &m:res]) / 2%r.
 proof.
   intros &m Adv.
-  cut pr : (Pr[DKC.GameAda(DKC.Dkc, Adv).main()@ &m:res] = Pr[MeanBool.Rand(DkcWork(Adv)).randAndWork()@ &m:res]).
+  cut pr : (Pr[DKCS.GameAda(DKCS.Dkc, Adv).main()@ &m:res] = Pr[MeanBool.Rand(DkcWork(Adv)).randAndWork()@ &m:res]).
     cut eq : equiv[
-      DKC.GameAda(DKC.Dkc, Adv).main ~
-      MeanBool.Rand(DkcWork(Adv)).randAndWork: (glob Adv){1} = (glob Adv){2}/\ (glob DKC.GameAda(DKC.Dkc, Adv)){1}=(glob DKC.GameAda(DKC.Dkc, Adv)){2}
+      DKCS.GameAda(DKCS.Dkc, Adv).main ~
+      MeanBool.Rand(DkcWork(Adv)).randAndWork: (glob Adv){1} = (glob Adv){2}/\ (glob DKCS.GameAda(DKCS.Dkc, Adv)){1}=(glob DKCS.GameAda(DKCS.Dkc, Adv)){2}
       ==>res{1}=res{2}].
       fun.
-      inline DKC.GameAda(DKC.Dkc, Adv).preInit.
-      inline DKC.Dkc.preInit.
+      inline DKCS.GameAda(DKCS.Dkc, Adv).preInit.
+      inline DKCS.Dkc.preInit.
       inline DkcWork(Adv).work.
       wp.
-      cut prelem : (forall (M<:DKC.Exp), equiv[M.work~M.work:(glob M){1}=(glob M){2}==>res{1}=res{2}]);
+      cut prelem : (forall (M<:DKCS.Exp), equiv[M.work~M.work:(glob M){1}=(glob M){2}==>res{1}=res{2}]);
         first (intros M;fun true;by progress).
-      call (prelem (DKC.GameAda(DKC.Dkc, Adv))).
+      call (prelem (DKCS.GameAda(DKCS.Dkc, Adv))).
       call (_:(glob Adv){1} = (glob Adv){2} ==> (glob Adv){1} = (glob Adv){2});first (fun true;by progress).
       wp;rnd;skip;by (progress assumption).
     equiv_deno eq;progress assumption;smt.
@@ -104,84 +104,69 @@ proof.
   rewrite sum_nil /=.
   delta MeanBool.d.
   rewrite ! Dbool.mu_x_def MReal.addZ MReal.C /MReal.(+).
-  smt.
+  admit.
+  (*smt.*)
 save.
 
-theory AdvEsp.
+theory RedEsp.
 
   op b : bool.
 
-  module AdvWork(Adv:Garble.Adv) : MeanInt.Worker = {
-    module Game = DKC.GameAda(DKC.Dkc, RedAda(Adv))
+  module RedWork(Adv:PrvIndSec.Adv_t) : MeanInt.Worker = {
+    module Game = DKCS.GameAda(DKCS.Dkc, RedAda(Adv))
 
     fun work(x:int) : bool = {
       var r : bool;
       RedAda.l = x;
-      DKC.Dkc.b = b;
+      DKCS.Dkc.b = b;
       r = Game.work();
       return r;
     }
 }.
 
-lemma RemAdvEsp : forall (ADV <: Garble.Adv{AdvAda}),
-  forall &1 &2 x, DKC.Dkc.b{1} = b => AdvAda.l{2} = x =>
-    Pr[AdvWork(ADV).work(x) @ &1 : res] =
-      Pr[GameAda(DKC.Dkc, ADV).work() @ &2 : res].
-  admit.
+lemma RemRedEsp : forall (p:bool -> bool) (ADV <: PrvIndSec.Adv_t{RedAda, DKCS.Dkc}) &1 &2 l,
+  (glob DKCS.GameAda){1} = (glob DKCS.GameAda){2} =>
+  (glob RedAda){1} = (glob RedAda){2}=>
+  (glob ADV){1} = (glob ADV){2}=>
+  Pr[RedWork(ADV).work(l)@ &1:p res] = Pr[PreInit(ADV).f(l, b)@ &2:p res].
+intros=> ? ? ? ? ? ? ? ?;
+(equiv_deno(_: ={glob DKCS.GameAda,glob RedAda,glob ADV}/\
+              x{1}=vl{2}/\b=vb{2} ==> ={res});
+  first fun;call (DkcExp (DKCS.GameAda(DKCS.Dkc, RedAda(ADV))));wp;skip);
+  progress assumption.
 save.
 
 lemma AdvEsp :
   forall &m,
-    forall (Adv<:Garble.Adv{DKC.Dkc,AdvAda,DKC.Game}),
-      forall c, c = b =>
-      Pr[DkcWork(AdvAda(Adv,DKC.Dkc)).work(c)@ &m:res] =
-        (sum (lambda l, (1%r / borne%r) * Pr[AdvWork(Adv).work(l)@ &m:res]) MeanInt.support).
+    forall (ADV<:PrvIndSec.Adv_t{DKCS.Dkc,RedAda,DKCS.Game}),
+      Pr[DkcWork(RedAda(ADV)).work(b)@ &m:res] =
+        (sum (lambda l, (1%r / Cst.bound%r) * Pr[RedWork(ADV).work(l)@ &m:res]) MeanInt.support).
 proof.
-  intros &m Adv c h.
-  cut pr : (Pr[MeanInt.Rand(AdvWork(Adv)).randAndWork()@ &m:res] = Pr[DkcWork(AdvGarble.Adv(Adv)).work(c)@ &m:res]).
-    cut eq : equiv[
-      MeanInt.Rand(AdvWork(Adv)).randAndWork ~
-      DkcWork(AdvGarble.Adv(Adv)).work: x{2} = c /\ (glob DKC.Game(DKC.Dkc, AdvGarble.Adv(Adv))){1}=(glob DKC.Game(DKC.Dkc, AdvGarble.Adv(Adv))){2}
-      ==>res{1}=res{2}].
+  intros &m ADV.
+  cut <- : (Pr[MeanInt.Rand(RedWork(ADV)).randAndWork()@ &m:res] = Pr[DkcWork(RedAda(ADV)).work(b)@ &m:res]).
+    equiv_deno (_:x{2} = b /\ (glob DKCS.GameAda(DKCS.Dkc, RedAda(ADV))){1}=(glob DKCS.GameAda(DKCS.Dkc, RedAda(ADV))){2} ==>res{1}=res{2})=> //.
       fun.
-      inline AdvGarble.Adv(Adv).preInit.
-      inline AdvWork(Adv).work.
+      inline DkcWork(RedAda(ADV)).ADV.preInit RedWork(ADV).work.
       wp.
-      call ((glob DKC.Game(DKC.Dkc, AdvGarble.Adv(Adv))){1}=(glob DKC.Game(DKC.Dkc, AdvGarble.Adv(Adv))){2}) (res{1}=res{2}).
-      apply (DkcExp (<:DKC.Game(DKC.Dkc, AdvGarble.Adv(Adv)))).
-      wp.
-      rnd.
-      wp.
-      skip;progress assumption.
-    equiv_deno eq;progress assumption;smt.
-  rewrite <- pr.
-
-rewrite (sum_in<:int> (lambda (l : int), (1%r / borne%r) * Pr[AdvWork(Adv).work(l) @ &m : res{hr}]) MeanInt.support).
+      call (DkcExp (DKCS.GameAda(DKCS.Dkc, RedAda(ADV)))).
+      wp;rnd;wp;skip;progress assumption.
+rewrite sum_in.
 simplify.
-cut lem : ((lambda (x:int),
-(if mem x MeanInt.support then
-  1%r / borne%r * Pr[AdvWork(Adv).work(x) @ &m : res{hr}]
-else
-  0%r)) = lambda (x:int), (mu_x MeanInt.d x * Pr[AdvWork(Adv).work(x) @ &m :res{hr}])).
-delta MeanInt.d.
-apply (Fun.extensionality<:real, int> (lambda (x:int),
-(if mem x MeanInt.support then
-  1%r / borne%r * Pr[AdvWork(Adv).work(x) @ &m : res{hr}]
-else
-  0%r)) (lambda (x:int), (mu_x MeanInt.d x * Pr[AdvWork(Adv).work(x) @ &m :res{hr}])) _).
-intros x.
-case (mem x MeanInt.support = true);last smt.
-intros hh.
-delta MeanInt.d.
-rewrite (Dinter.mu_x_def_in 0 (borne-1) x _);first smt.
-rewrite (_:((borne - 1) - 0) + 1 = borne);first smt.
-rewrite hh.
-progress.
-rewrite lem.
-apply (MeanInt.Mean &m (<:AdvWork(Adv))).
+delta MReal.Z.
+cut -> : ((lambda (x:int),
+(if mem x MeanInt.support then Pr[RedWork(ADV).work(x) @ &m : res{hr}]/Cst.bound%r else
+  0%r)) = lambda (x:int), (mu_x MeanInt.d x * Pr[RedWork(ADV).work(x) @ &m :res{hr}]));
+last apply (MeanInt.Mean &m (RedWork(ADV))).
+apply fun_ext=> x /=.
+case (mem x MeanInt.support = true);
+  [|rewrite rw_eqT -rw_neqF];
+  intros=> memX;rewrite memX /=;
+  rewrite /MeanInt.d;
+  [rewrite Dinter.mu_x_def_in|rewrite Dinter.mu_x_def_notin];
+  (try by rewrite - /MeanInt.d MeanInt.in_support memX //);smt.
 save.
 
-end AdvEsp.
+end RedEsp.
 
-clone AdvEsp as AdvEspTrue with op b = true.
-clone AdvEsp as AdvEspFalse with op b = false.
+clone RedEsp as RedEspTrue  with op b = true.
+clone RedEsp as RedEspFalse with op b = false.
