proof/garbleTools.ec
@@ -6,6 +6,7 @@ require import Int.
 require import Pair.
 require import Bool.
 
+require import MyTools.
 
 type token = bitstring.
 type tokens = (token*token) array.
@@ -58,7 +59,6 @@ rewrite ! Bits.cons_inj=> [[? ?] ?].
 subst;split=> //.
 apply intToBitstring_inj=> //.
 save.
-
 
 op evalGate(f:'a gate, i:bool*bool) : 'a =
   let (ff, ft, tf, tt) = f in
@@ -128,4 +128,103 @@ proof.
   simplify evalGate garbleGate enc.
   generalize H5.
   case (! lsb gi1 && ! lsb gi2)=> h;smt.
+save.
+
+
+type w2g = int array.
+type 'a g2v = ('a*'a*'a*'a) array.
+type 'a functGen = int*int*int*w2g*w2g*('a g2v).
+
+(*Access to funct member*)
+op getN(f:'a functGen) : int =
+  let (n, m, q, a, b, g) = f in n.
+op getM(f:'a functGen) : int =
+  let (n, m, q, a, b, g) = f in m.
+op getQ(f:'a functGen) : int =
+  let (n, m, q, a, b, g) = f in q.
+op getA(f:'a functGen) : w2g =
+  let (n, m, q, a, b, g) = f in a.
+op getB(f:'a' functGen) : w2g =
+  let (n, m, q, a, b, g) = f in b.
+op getG(f:'a functGen) : 'a g2v =
+  let (n, m, q, a, b, g) = f in g.
+
+op evalComplete(f:'a functGen, x:'a array, extract:'a functGen -> int -> 'a array -> 'a) : 'a array =
+  appendInit x ((getN f)+(getQ f)) (extract f).
+
+op evalGen(f:'a functGen, x:'a array, extract:'a functGen -> int -> 'a array -> 'a) : 'a array =
+  Array.sub (evalComplete f x extract) ((getN f) + (getQ f) - (getM f)) (getM f).
+
+op extract(f:bool functGen, g:int, x:bool array) : bool =
+  evalGate (getG f).[g] (x.[(getA f).[g]], x.[(getB f).[g]]).
+
+  
+op extractG(ff:token functGen, g:int, x:token array) =
+  let a = (getA ff).[g] in
+  let b = (getB ff).[g] in
+  let aA = x.[a] in
+  let bB = x.[b] in
+  let a = lsb aA in
+  let b = lsb bB in
+  let t = tweak g a b in
+  DKC.decode t aA bB (evalGate ((getG ff).[g]) (a, b)).
+
+
+op garbMap(x:tokens, f:bool functGen, g:int) : token*token*token*token =
+  garbleGate x (getG f).[g] (getA f).[g] (getB f).[g] g.
+
+op choose(k:(token*token) array, i:bool array, j:int) : token = getTok k j i.[j].
+
+op validCircuit(bound:int, f:(bool functGen)) =
+  let (n, m, q, aa, bb, gg) = f in
+  n > 1 /\ m > 0 /\ q > 0 /\ q >= m /\
+  n + q - m = bound /\
+  length aa = n + q /\ length bb = n + q /\ length gg = n + q /\
+  (range n (n+q) true (lambda i b, b /\ aa.[i] >= 0 /\ bb.[i] < i /\ bb.[i] < n+q-m /\ aa.[i] < bb.[i])).
+
+lemma valid_wireinput :
+  forall (bound:int) (f:(bool functGen)),
+    validCircuit bound f <=> 
+  let (n, m, q, aa, bb, gg) = f in
+  n > 1 /\ m > 0 /\ q > 0 /\ q >= m /\
+  n + q - m = bound /\
+  Array.length aa = n + q /\ Array.length bb = n + q /\ Array.length gg = n + q /\
+      (forall i,
+         i >= n  => i < n+q =>
+           aa.[i] >= 0 /\
+           bb.[i] < i /\
+           bb.[i] < n+q-m /\
+           aa.[i] < bb.[i]).
+delta validCircuit.
+intros f.
+elimT tuple6_ind f.
+intros n m q aa bb gg valF.
+case (n > 1);last simplify;smt.
+case (m > 0);last simplify;split.
+case (q > 0);last simplify;split.
+case (n + q - m = bound);last simplify;split.
+case (length aa = n + q);last simplify;split.
+case (length bb = n + q);last simplify;split.
+case (length gg = n + q);last simplify;split.
+intros H1 H2 H3 H4 H5 H6 H7.
+rewrite (_:(n > 1) = true);first smt.
+simplify.
+apply (_:forall a b d, (b <=> d) => (a /\ b <=> a /\ d));first smt.
+pose {1 3} j := q.
+elim/Induction.induction j;last first;first 2 smt.
+simplify => k hypJ hypRec.
+rewrite range_ind;first smt.
+rewrite (_:(n + k - 1 = n + (k - 1)));first smt.
+rewrite hypRec.
+simplify.
+split => h.
+elim h => h1 h2 i.
+case (i = n + (k - 1)).
+  intros => -> _ _.
+apply h2.
+intros hh1 hh2 hh3.
+apply h1.
+assumption.
+smt.
+(split;first intros i hI hI2);apply h;smt.
 save.
