proof/garble.ec
@@ -1,0 +1,64 @@
+require import Real.
+require import Pair.
+require import Bool.
+require import INDCPA.
+
+theory Garble.
+  type funct.
+  type functG.
+  type input.
+  type output.
+  type keyInput.
+  type keyOutput.
+  type inputG.
+  type outputG.
+  type tPhi.
+  
+  type random.
+
+  op functCorrect : funct -> bool.
+  op inputCorrect : funct -> input -> bool.
+  (*pred randomCorrect : (funct, random).*)
+
+  op garble : random -> funct -> functG*keyInput*keyOutput.
+  op encrypt : keyInput -> input -> inputG.
+  op decrypt : keyOutput -> outputG -> output.
+  op eval : funct -> input -> output.
+  op evalG : functG -> inputG -> outputG.
+  op phi : funct -> tPhi.
+  op phiG : functG -> tPhi.
+end Garble.
+
+theory Correct.
+  clone import Garble.
+
+  axiom Correct : forall (f:funct) (x:random) (i:input),
+    functCorrect f =>
+    (*randomCorrect f x =>*)
+    inputCorrect f i =>
+      let (g, ki, ko) = garble x f in
+      eval f i = decrypt ko (evalG g (encrypt ki i)).
+end Correct.
+
+theory PrvInd.
+  clone import Garble.
+
+  clone INDCPA_Scheme with
+    type query = funct*input,
+    type answer = functG*inputG*keyOutput,
+    type random = random,
+
+    op queryValid(queries:query*query) =
+      let query0 = fst queries in
+      let query1 = snd queries in
+      functCorrect (fst query0) /\ functCorrect (fst query1) /\
+      inputCorrect (fst query0) (snd query0) /\ inputCorrect (fst query1) (snd query1) /\
+      eval (fst query0) (snd query0) = eval (fst query1) (snd query1) /\
+      phi (fst query0) = phi (fst query1),
+
+    op work (q:query) (r:random) =
+      let (f, x) = q in
+      let (g, ki, ko) = garble r f in
+      (g, encrypt ki x, ko).
+
+end PrvInd.
