proof/garble/preProof.ec
@@ -1,0 +1,34 @@
+require import Int.
+
+require Dkc.
+require GarbledCircuit.
+require INDCPA.
+
+(* Security parameter and bound on circuit size*)
+theory Cst.
+op k : int.
+axiom kVal : k > 1.
+
+op bound : int.
+axiom boundInf : bound > 1.
+end Cst.
+
+(* Take a semi concrete DKC *)
+clone Dkc.DKC as DKC with
+  op k = Cst.k
+  proof kVal by apply Cst.kVal.
+
+(* Definition of security of DKC *)
+clone Dkc.DKC_Sec as DKCS with
+  theory DKC_Abs = DKC.
+
+(* Take a GarbleCircuit *)
+clone export GarbledCircuit as GC with
+  theory Cst = Cst,
+  theory DKC = DKC.
+
+(* We want to prove PrvInd security base on INDCPA *)
+clone Garble.PrvInd as PrvInd_Circuit with
+  theory Garble = GC.GarbleCircuit.
+clone INDCPA.INDCPA_Def as PrvIndSec with
+  theory INDCPA_Scheme = PrvInd_Circuit.INDCPA_Scheme.
